# 3.2 Iterative Method

- Expand the recurrence step by step until a clear pattern emerges.
- Replace the recurrence with successive substitutions.
- Stop once the base case is reached, then simplify.

!!! note "**Example 1:**"

      $$ T(n) = T(n-1) + 1, \quad T(1) = 1 $$

      Weâ€™ll solve it by **unrolling** (expanding) step by step until the base case.

      **Step 1. Unroll the Recurrence**

      Start expanding:

      $$ T(n) = T(n-1) + 1 $$

      $$ T(n-1) = T(n-1-1) + 1  \quad\implies\quad T(n) = T(n-2) + 2 $$

      $$ T(n-2) = T(n-2-1) + 1 + 1 \quad\implies\quad T(n) = T(n-3) + 3 $$

      $$ T(n-3) = T(n-3-1) + 1 + 1 + 1 + 1 \quad\implies\quad T(n) = T(n-4) + 4 $$

      After \(k\) steps, the pattern is:

      $$      T(n) = T(n-k) + k $$


      **Step 2. Stop at the Base Case**

      Pick \(k\) so that \(n - k\) hits the base index \(b\) (where \(b=1\) in this case):


      $$ n - k = 1 \quad\Rightarrow\quad k = n - 1 $$

      Now substitute \(k = n - 1\) into the pattern:

      $$
      T(n) = T(1) + (n - 1)
      $$

      **Step 3. Plug In Your Base**

      $$
      T(n) = T(1) + (n-1) \newline
            = 1 + (n-1)
      $$

     $ \therefore $ the growth is **linear**.


      **step 4. Final Result (Asymptotics)**

      $$
      \boxed{T(n) = \Theta(n)}
      $$

      **Intuition:** each step reduces \(n\) by 1 and adds a constant cost \(+1\), so the total work scales linearly with \(n\).

---

#### Try this Question

??? question " Q1. $ \quad T(n) = T(n-1)+n, \quad T(1) = 1 $ "

      $$ T(n) = T(n-1)+n, \quad T(1) = 1 $$

      **Step 1. Unroll the Recurrence**

      Start expanding:

      $$ T(n) = T(n-1) + n $$

      $$ T(n-1) = T(n-1-1) + n-1  \quad\implies\quad T(n) = (T(n-2) + n-1) + n $$

      $$ T(n-2) = T(n-2-1) + n-2 \quad\implies\quad T(n) = ((T(n-3)+ n-2) + n-1) + n $$

      $$ T(n-3) = T(n-3-1) + n-3  \quad\implies\quad T(n) = ((T(n-4)+n-3)+n-2)+n-1+n $$

      After \(k\) steps, the pattern is:

      $$      T(n) = T(n-k) + (n-k+1) + (n-k+2) + (n-k+3) ... n $$

      **Step 2. Stop at the Base Case**

      Pick \(k\) so that \(n - k\) hits the base index 1:


      $$ n - k = 1 \quad\Rightarrow\quad k = n - 1 $$

      Now substitute \(k = n - 1\) into the pattern:

      $$
      T(n) = T(1) + 2 +3 + 4 +...+n
      $$

      **Step 3. Plug In Your Base**

      $$
      T(n) = T(1) + 2 + 3 + 4 + ... + (n-1) + n \newline
            = 1 + 2 + 3 + 4 + ... + n
      $$

     Since we can observe that the algorithm tends to behave as a sum of first \(n\) integers

     $$ 1 + 2 + 3 + 4 + ... + n = \frac{n(n+1)}{2} $$

     So,
     $$ T(n) = \frac{n(n+1)}{2} $$

     **step 4. Final Result (Asymptotics)**

      $$
      \boxed{T(n) = \Theta(n^2)}
      $$

<!-- Second Question -->

??? question " Q2. $ \quad T(n) = T(n/2)+1, \quad T(1) = 1 $ "

      $$ T(n) = T(n/2)+1, \quad T(1) = 1 $$

      **Step 1. Unroll the Recurrence**

      Start expanding:

      $$ T(n) = T(n/2) + 1 $$

      $$ T(n/2) = T(n/4) + 1  \quad\implies\quad T(n) = T(n/4) +  2 $$

      $$ T(n/4) = T(n/8) + 2 \quad\implies\quad T(n) = T(n/8)+ 3 $$

      $$ T(n/8) = T(n/16) + 3  \quad\implies\quad T(n) = T(n/16) + 4 $$

      After \(k\) steps, the pattern is:

      $$      T(n) = T(n/2^k) + k $$

      **Step 2. Stop at the Base Case**

      Pick \(k\) so that \(n/2^k\) hits the base index 1:


      $$ n/2^k = 1 \quad\Rightarrow\quad k = c . log n $$

      Now substitute \(k = clog n\) into the pattern:

      $$
      T(n) = T(1) + c.log n
      $$

      **Step 3. Plug In Your Base**

      $$
      T(n) = T(1) + c.log n \newline
            = 1 + c.logn
      $$


     **step 4. Final Result (Asymptotics)**

      $$
      \boxed{T(n) = \Theta (logn)}
      $$
